theories/tree_borrows/tag_protected_laws.v
@@ -10,17 +10,19 @@ From simuliris.tree_borrows Require Import tree_access_laws logical_state inv_ac
 From iris.prelude Require Import options.
 
 (* TODO move somewhere else *)
-Lemma tag_protected_preserved_by_access_strong tg_acc tg_prs l C c trs trs' acc blk off sz b :
+Lemma tag_protected_preserved_by_access_strong tg_acc tg_prs l C c trs trs' acc blk off sz b P ae:
   wf_trees trs →
   apply_within_trees (memory_access_maybe_nonchildren_only b acc C tg_acc (off, sz)) blk trs = Some trs' →
   call_is_active c C →
-  tag_protected_for c trs  l tg_prs ProtStrong →
-  tag_protected_for c trs' l tg_prs ProtStrong.
+  tag_protected_for P c trs  l tg_prs (EnsuringAccess ae) →
+  tag_protected_for P c trs' l tg_prs (EnsuringAccess ae).
 Proof.
   intros Hwf Hwithin Hcall (it & Hlu & Hprot & Hstrong & Hinit).
   destruct (decide (l.1 = blk ∧ (off ≤ l.2 < off + sz))%Z) as [(<- & Hin)|Hout].
-  - eapply apply_trees_access_lookup_general in Hlu as (itnew & Hlunew & Heqinit & Heqprot & Hacc); [|done..].
+  - pose proof Hlu as Hlu2. eapply apply_trees_access_lookup_general in Hlu2 as (itnew & Hlunew & Heqinit & Heqprot & Hacc); [|done..].
     exists itnew. split; first done. rewrite /item_protected_for -Heqprot.
+    assert (itag it = itag itnew) as Heqitag by by repeat erewrite trees_lookup_correct_tag.
+    rewrite -Heqitag. 
     do 2 (split; first done).
     intros Hperminit.
     assert (protector_is_active (iprot itnew) C) as Hactive.
@@ -38,17 +40,20 @@ Proof.
       [ specialize (Hinit eq_refl) | ].
     all: destruct trees_rel_dec eqn:Hreldec; destruct acc; destruct (perm (item_lookup it l.2)) as [[] []| | |] eqn:Hpermold; simpl in *; simplify_eq; try done;
          repeat (simplify_eq; try done; (try simpl in Htrigger); simplify_eq; try done).
-  - eapply apply_trees_access_lookup_outside in Hlu as (itnew & Hlunew & Heqinit & Heqprot & Hacc); [|done..].
+  - eapply apply_trees_access_lookup_outside in Hlu as Hlu2; [|done..].
+    destruct Hlu2 as (itnew & Hlunew & Heqinit & Heqprot & Hacc).
     exists itnew. split; first done. rewrite /item_protected_for -Heqprot.
+    assert (itag it = itag itnew) as Heqitag by by repeat erewrite trees_lookup_correct_tag.
+    rewrite -Heqitag. 
     do 2 (split; first done).
     by rewrite -Hacc.
 Qed.
-Lemma tag_protected_preserved_by_access_weak tg_acc tg_prs l C c trs trs' acc blk off sz b :
+Lemma tag_protected_preserved_by_access_weak tg_acc tg_prs l C c trs trs' acc blk off sz b P :
   wf_trees trs →
   apply_within_trees (memory_access_maybe_nonchildren_only b acc C tg_acc (off, sz)) blk trs = Some trs' →
   call_is_active c C →
-  tag_protected_for c trs  l tg_prs ProtWeak →
-  tag_protected_for c trs' l tg_prs ProtWeak.
+  tag_protected_for P c trs  l tg_prs Deallocable →
+  tag_protected_for P c trs' l tg_prs Deallocable.
 Proof.
   intros Hwf Hwithin Hcall Hold it Hlu.
   destruct (decide (l.1 = blk ∧ (off ≤ l.2 < off + sz))%Z) as [(<- & Hin)|Hout].
@@ -74,58 +79,64 @@ Proof.
     do 2 (split; first done).
     by rewrite -Hacc.
 Qed.
-Lemma tag_protected_preserved_by_access tg_acc tg_prs l C c trs trs' acc blk off sz b ps:
+Lemma tag_protected_preserved_by_access tg_acc tg_prs l C c trs trs' acc blk off sz b ps P:
   wf_trees trs →
   apply_within_trees (memory_access_maybe_nonchildren_only b acc C tg_acc (off, sz)) blk trs = Some trs' →
   call_is_active c C →
-  tag_protected_for c trs  l tg_prs ps →
-  tag_protected_for c trs' l tg_prs ps.
+  tag_protected_for P c trs  l tg_prs ps →
+  tag_protected_for P c trs' l tg_prs ps.
 Proof.
   destruct ps.
-  - eapply tag_protected_preserved_by_access_strong.
   - eapply tag_protected_preserved_by_access_weak.
+  - eapply tag_protected_preserved_by_access_strong.
 Qed.
 
 (* TODO move somewhere else *)
-Lemma tag_protected_preserved_by_delete tg_acc tg_prs l C c trs trs' blk off sz ps :
+Lemma tag_protected_preserved_by_delete tg_acc tg_prs l C c trs trs' blk off sz ps P :
   wf_trees trs →
   apply_within_trees (memory_deallocate C tg_acc (off, sz)) blk trs = Some trs' →
   call_is_active c C →
-  tag_protected_for c trs l tg_prs ps →
-  tag_protected_for c (delete blk trs') l tg_prs ps.
+  (∀ it, ps = EnsuringAccess WeaklyNoChildren → l.1 = blk → trees_lookup trs blk tg_prs it → P tg_prs l → protector_is_for_call c (iprot it) → (initialized (item_lookup it l.2) = PermInit → perm (item_lookup it l.2) ≠ Disabled) → False) →
+  tag_protected_for P c trs l tg_prs ps →
+  tag_protected_for P c (delete blk trs') l tg_prs ps.
 Proof.
-  intros Hwf Hwithin Hcall Hpreprot.
+  intros Hwf Hwithin Hcall HPprotect Hpreprot.
   rewrite apply_within_trees_bind in Hwithin.
   pose proof Hwithin as (postread&Hread&Hdealloc)%bind_Some.
   eapply tag_protected_preserved_by_access in Hread as HH. 2-4: done.
-  destruct (decide (l.1 = blk)) as [<-|Hout], ps.
+  destruct (decide (l.1 = blk)) as [<-|Hout], ps as [|ae].
+  - clear HH. intros it (tr&Htr&Hit). by rewrite lookup_delete in Htr.
   - exfalso. destruct HH as (it & (tr & Htr & Hlu) & Hprot & Hstrong & Hinit).
+    destruct ae; last first.
+    { destruct Hpreprot as (it' & (tr' & Htr' & Hlu') & Hprot' & Hstrong' & Hinit'). destruct l.
+      erewrite tree_lookup_correct_tag in Hstrong'; last done. 
+      eapply HPprotect. 1: done. 3: exact Hstrong'. 1: done. 1: eexists; split; first done. 2: eapply Hprot'. 1: eapply Hlu'. done.
+    }
     rewrite /apply_within_trees Htr /= in Hdealloc.
     pose proof Hdealloc as (okcheck&Hcheck%mk_is_Some&[= <-])%bind_Some. clear Hdealloc.
     rewrite join_success_condition every_node_map every_node_eqv_universal /= in Hcheck.
     pose proof (tree_lookup_correct_tag Hlu) as <-.
     ospecialize (Hcheck it _); first by eapply tree_lookup_to_exists_node.
-    eapply is_Some_if_neg in Hcheck. ospecialize (Hstrong _); first done.
+    eapply is_Some_if_neg in Hcheck.
     rewrite (bool_decide_eq_true_2 _ Hstrong) /=bool_decide_eq_false in Hcheck.
     eapply Hcheck.
     exists c. done.
-  - clear HH. intros it (tr&Htr&Hit). by rewrite lookup_delete in Htr.
+  - intros it (tr&(Hne&Hin)%lookup_delete_Some&Hit).
+    eapply HH. exists tr. split; last done.
+    eapply bind_Some in Hdealloc as (tr1&Htr1&(tr2&Htr2&[= Heq])%bind_Some).
+    rewrite -Heq lookup_insert_ne // in Hin.
   - destruct HH as (it & (tr & Htr & Hlu) & Hprot & Hstrong & Hinit).
     exists it. split; last done. exists tr. split; last done.
     rewrite lookup_delete_ne //.
     pose proof Hdealloc as (?&_&(?&_&[= <-])%bind_Some)%bind_Some.
     by rewrite lookup_insert_ne.
-  - intros it (tr&(Hne&Hin)%lookup_delete_Some&Hit).
-    eapply HH. exists tr. split; last done.
-    eapply bind_Some in Hdealloc as (tr1&Htr1&(tr2&Htr2&[= Heq])%bind_Some).
-    rewrite -Heq lookup_insert_ne // in Hin.
 Qed.
 
-Lemma tag_protected_preserved_by_create_strong tg_par tg_cld pk rk C cc c trs trs' blk l tg_prs:
+Lemma tag_protected_preserved_by_create_strong tg_par tg_cld pk rk C cc c trs trs' blk l tg_prs P ae:
   wf_trees trs → tg_cld ≠ tg_prs →
   apply_within_trees (create_child C tg_par tg_cld pk rk cc) blk trs = Some trs' →
-  tag_protected_for c trs  l tg_prs ProtStrong →
-  tag_protected_for c trs' l tg_prs ProtStrong.
+  tag_protected_for P c trs  l tg_prs (EnsuringAccess ae) →
+  tag_protected_for P c trs' l tg_prs (EnsuringAccess ae).
 Proof.
   intros Hwf Hncontain (tr&Htr&(tr'&Hcreate&[= <-])%bind_Some)%bind_Some (it & Hlu & Hprot & Hstrong & Hinit).
   exists it. split; last done. destruct Hlu as (tt&Htt&Hit).
@@ -138,11 +149,11 @@ Proof.
   - eapply create_child_preserves_determined. 2: apply Hlu. 2: eapply Hcreate.
     by intros ->.
 Qed.
-Lemma tag_protected_preserved_by_create_weak tg_par tg_cld pk rk C cc c trs trs' blk l tg_prs:
+Lemma tag_protected_preserved_by_create_weak tg_par tg_cld pk rk C cc c trs trs' blk l tg_prs P:
   wf_trees trs → tg_cld ≠ tg_prs →
   apply_within_trees (create_child C tg_par tg_cld pk rk cc) blk trs = Some trs' →
-  tag_protected_for c trs  l tg_prs ProtWeak →
-  tag_protected_for c trs' l tg_prs ProtWeak.
+  tag_protected_for P c trs  l tg_prs Deallocable →
+  tag_protected_for P c trs' l tg_prs Deallocable.
 Proof.
   intros Hwf Hncontain (tr&Htr&(tr'&Hcreate&[= <-])%bind_Some)%bind_Some Hprot it Hlu.
   eapply Hprot. destruct Hlu as (tt&Htt&Hit).
@@ -157,46 +168,45 @@ Proof.
     eapply insert_true_preserves_every. 2: apply Hlu.
     simpl. intros ->; done.
 Qed.
-Lemma tag_protected_preserved_by_create ps tg_par tg_cld pk rk C cc c trs trs' blk l tg_prs:
+Lemma tag_protected_preserved_by_create ps tg_par tg_cld pk rk C cc c trs trs' blk l tg_prs P:
   wf_trees trs → tg_cld ≠ tg_prs →
   apply_within_trees (create_child C tg_par tg_cld pk rk cc) blk trs = Some trs' →
-  tag_protected_for c trs  l tg_prs ps →
-  tag_protected_for c trs' l tg_prs ps.
+  tag_protected_for P c trs  l tg_prs ps →
+  tag_protected_for P c trs' l tg_prs ps.
 Proof.
   destruct ps.
-  - eapply tag_protected_preserved_by_create_strong.
   - eapply tag_protected_preserved_by_create_weak.
+  - eapply tag_protected_preserved_by_create_strong.
 Qed.
 
 
+Definition tag_protected_for_tree P c tr l t ps := match ps with
+  | Deallocable   => ∀ it, tree_lookup tr t it → item_protected_for P c it l.1 l.2 ps
+  | EnsuringAccess _ => ∃ it, tree_lookup tr t it ∧ item_protected_for P c it l.1 l.2 ps end.
 
-Definition tag_protected_for_tree c tr off t (ps : prot_strong) := match ps with
-    ProtStrong => ∃ it, tree_lookup tr t it ∧ item_protected_for c it off ps
-  | ProtWeak   => ∀ it, tree_lookup tr t it → item_protected_for c it off ps end.
-
-Lemma tag_protected_for_tree_spec trs tr blk c off t ps :
-  trs !! blk = Some tr →
-  tag_protected_for_tree c tr off t ps ↔ tag_protected_for c trs (blk, off) t ps.
+Lemma tag_protected_for_tree_spec trs tr c l t ps P :
+  trs !! l.1 = Some tr →
+  tag_protected_for_tree P c tr l t ps ↔ tag_protected_for P c trs l t ps.
 Proof.
   intros H.
   destruct ps; split.
-  - intros (it&H1&HH). exists it. split; last done. eexists. simpl. done.
-  - intros (it&(tr'&H1&H2)&HH). exists it; split; last done. rewrite /= H in H1. by injection H1 as ->.
   - intros HH it (tr'&Htr&Hit). eapply HH. rewrite /= H in Htr. congruence.
   - intros HH it Hit. eapply HH. exists tr. simpl. done.
+  - intros (it&H1&HH). exists it. split; last done. eexists. simpl. done.
+  - intros (it&(tr'&H1&H2)&HH). exists it; split; last done. rewrite /= H in H1. by injection H1 as ->.
 Qed.
 
-Lemma tag_protected_preserved_by_access_tree tg_acc tg_prs loff C c tr tr' acc off sz b ps :
+Lemma tag_protected_preserved_by_access_tree tg_acc tg_prs loff C c tr tr' acc off sz b ps P :
   wf_tree tr →
   memory_access_maybe_nonchildren_only b acc C tg_acc (off, sz) tr = Some tr' →
   call_is_active c C →
-  tag_protected_for_tree c tr loff tg_prs ps →
-  tag_protected_for_tree c tr' loff tg_prs ps.
+  tag_protected_for_tree P c tr loff tg_prs ps →
+  tag_protected_for_tree P c tr' loff tg_prs ps.
 Proof.
   intros H1 H2 H3 H4.
-  eapply wf_tree_wf_singleton in H1.
-  eassert ({[1%positive := tr]} !! _ = Some tr) as Hlu by eapply lookup_singleton.
-  eassert ({[1%positive := tr']} !! _ = Some tr') as Hlu' by eapply lookup_singleton.
+  eapply wf_tree_wf_singleton_any in H1.
+  eassert ({[loff.1 := tr]} !! _ = Some tr) as Hlu by eapply lookup_singleton.
+  eassert ({[loff.1 := tr']} !! _ = Some tr') as Hlu' by eapply lookup_singleton.
   setoid_rewrite tag_protected_for_tree_spec; last done.
   eapply tag_protected_preserved_by_access. 1: done. 2: done.
   - rewrite /apply_within_trees /=. setoid_rewrite Hlu. rewrite /=. erewrite H2.
@@ -204,13 +214,13 @@ Proof.
   - eapply tag_protected_for_tree_spec; done.
 Qed.
 
-Lemma tree_read_many_preserve_tag_protected_for_2 C tg_acc (L : list Z) tr1 trL c offp tg_prs ps
+Lemma tree_read_many_preserve_tag_protected_for_2 C tg_acc (L : list Z) tr1 trL c offp tg_prs ps P
   (Hwf1 : wf_tree tr1) :
   call_is_active c C →
   let fn := (λ L tr, foldr (λ l tr2, tr2 ≫= memory_access_nonchildren_only AccessRead C tg_acc (l, 1%nat)) (Some tr) L) in
   fn L tr1 = Some trL →
-  tag_protected_for_tree c tr1 offp tg_prs ps →
-  tag_protected_for_tree c trL offp tg_prs ps.
+  tag_protected_for_tree P c tr1 offp tg_prs ps →
+  tag_protected_for_tree P c trL offp tg_prs ps.
 Proof.
   intros Hact fn.
   induction L as [|off L IH] in trL|-*; simpl.
@@ -224,13 +234,13 @@ Proof.
   by eapply IH.
 Qed.
 
-Lemma tree_read_many_preserve_tag_protected_for_1 C (L : list (tag * gset Z)) tr1 trL c offp tg_prs ps
+Lemma tree_read_many_preserve_tag_protected_for_1 C (L : list (tag * gset Z)) tr1 trL c offp tg_prs ps P
   (Hwf1 : wf_tree tr1) :
   call_is_active c C →
   let fn := (λ E tr, foldr (λ '(tg, L) tr, tr ≫= λ tr1, foldr (λ l tr2, tr2 ≫= memory_access_nonchildren_only AccessRead C tg (l, 1%nat)) (Some tr1) (elements L)) (Some tr) E) in
   fn L tr1 = Some trL →
-  tag_protected_for_tree c tr1 offp tg_prs ps →
-  tag_protected_for_tree c trL offp tg_prs ps.
+  tag_protected_for_tree P c tr1 offp tg_prs ps →
+  tag_protected_for_tree P c trL offp tg_prs ps.
 Proof.
   intros Hact fn.
   induction L as [|(tg_acc&S) L IH] in trL|-*; simpl.
@@ -244,32 +254,25 @@ Proof.
   by eapply IH.
 Qed.
 
-Lemma tree_read_many_preserve_tag_protected_for C cid tr1 trL c offp tg_prs ps
+Lemma tree_read_many_preserve_tag_protected_for C cid tr1 trL c offp tg_prs ps P
   (Hwf1 : wf_tree tr1) :
   call_is_active c C →
   tree_read_all_protected_initialized C cid tr1 = Some trL →
-  tag_protected_for_tree c tr1 offp tg_prs ps →
-  tag_protected_for_tree c trL offp tg_prs ps.
+  tag_protected_for_tree P c tr1 offp tg_prs ps →
+  tag_protected_for_tree P c trL offp tg_prs ps.
 Proof.
   rewrite /tree_read_all_protected_initialized.
   rewrite /set_fold /=. eapply tree_read_many_preserve_tag_protected_for_1. done.
 Qed.
 
-Lemma trees_read_many_preserve_tag_protected_for C cid trs1 trsL c l tg_prs ps
+Lemma trees_read_many_preserve_tag_protected_for C cid trs1 trsL c l tg_prs ps P
   (Hwf1 : wf_trees trs1) :
   call_is_active c C →
   trees_read_all_protected_initialized C cid trs1 = Some trsL →
-  tag_protected_for c trs1 l tg_prs ps →
-  tag_protected_for c trsL l tg_prs ps.
+  tag_protected_for P c trs1 l tg_prs ps →
+  tag_protected_for P c trsL l tg_prs ps.
 Proof.
   intros H1 H2 H3. destruct l as [blk offl], ps.
-  - assert (∃ tr, trs1 !! blk = Some tr) as (tr&Htr).
-    { destruct H3 as (x&(tr&Htr&_)&_). by eexists. }
-    eapply trees_read_all_protected_initialized_pointwise_1 in H2 as (H2&_).
-    specialize (H2 _ Htr) as (tr'&Htr'&Hread).
-    eapply tag_protected_for_tree_spec. 1: done.
-    eapply tree_read_many_preserve_tag_protected_for. 1: by eapply Hwf1. 1: done. 1: done.
-    eapply tag_protected_for_tree_spec. all: done.
   - intros itL (trL&HtrL&HitL). simpl in HtrL.
     assert (∃ tr, trs1 !! blk = Some tr) as (tr&Htr).
     { eapply trees_read_all_protected_initialized_pointwise_1 in H2 as (_&H2B).
@@ -278,19 +281,26 @@ Proof.
     eapply trees_read_all_protected_initialized_pointwise_1 in H2 as (H2&_).
     specialize (H2 _ Htr) as (tr'&Htr'&Hread). assert (trL = tr') as -> by congruence. simpl.
     eapply tree_read_many_preserve_tag_protected_for in Hread; first last. 3: by eapply Hwf1. 2: done.
-    1: by eapply tag_protected_for_tree_spec.
+    1: eapply tag_protected_for_tree_spec; last exact H3. 1: by rewrite /=.
     eapply Hread. done.
+  - assert (∃ tr, trs1 !! blk = Some tr) as (tr&Htr).
+    { destruct H3 as (x&(tr&Htr&_)&_). by eexists. }
+    eapply trees_read_all_protected_initialized_pointwise_1 in H2 as (H2&_).
+    specialize (H2 _ Htr) as (tr'&Htr'&Hread).
+    eapply tag_protected_for_tree_spec. 1: done.
+    eapply tree_read_many_preserve_tag_protected_for. 1: by eapply Hwf1. 1: done. 1: done.
+    eapply tag_protected_for_tree_spec. all: done.
 Qed.
 
-Lemma call_set_interp_remove c M σ σ' :
+Lemma call_set_interp_remove c M σ σ' P :
   snc σ = snc σ' →
   snp σ = snp σ' →
   scs σ ∖ {[c]} = scs σ' →
   shp σ = shp σ' →
   state_wf σ →
   trees_read_all_protected_initialized (scs σ) c (strs σ) = Some (strs σ') →
-  call_set_interp M σ →
-  call_set_interp (delete c M) σ'.
+  call_set_interp P M σ →
+  call_set_interp P (delete c M) σ'.
 Proof.
   intros Heq1 Heq2 Heq3 Heq4 Heq5 Hwf Hinterp c' M' Hsome. destruct (decide (c' = c)) as [-> | Hneq].
   { rewrite lookup_delete in Hsome. done. }
@@ -304,5 +314,29 @@ Proof.
   eapply trees_read_many_preserve_tag_protected_for.
   3: done. 3: by eapply Hlookup. 1: by eapply state_wf_tree_unq.
   by eapply Hin.
+Qed.
+
+Lemma tag_protected_for_mono P1 P2 c trs l tg ps :
+  (∀ l it, trees_lookup trs l.1 tg it → protector_is_for_call c (iprot it) → (initialized (item_lookup it l.2) = PermInit → perm (item_lookup it l.2) ≠ Disabled) → P1 (itag it) l → P2 (itag it) l) →
+  tag_protected_for P1 c trs l tg ps →
+  tag_protected_for P2 c trs l tg ps.
+Proof.
+  intros Hweak H. destruct ps as [|[]].
+  1,2: rewrite /= /item_protected_for in H|-*; apply H.
+  destruct H as (it&Hit&Hprot&HP1&Hrst).
+  exists it. split; first done. split_and!; try done.
+  by eapply Hweak.
+Qed.
+
+Lemma call_set_interp_mono M σ P1 P2 :
+  (∀ tg c l it, call_is_active c σ.(scs) → trees_lookup σ.(strs) l.1 tg it → protector_is_for_call c (iprot it) → (initialized (item_lookup it l.2) = PermInit → perm (item_lookup it l.2) ≠ Disabled) → P1 (itag it) l → P2 (itag it) l) →
+  call_set_interp P1 M σ →
+  call_set_interp P2 M σ.
+Proof.
+  intros Hweak H1 c S HS.
+  specialize (H1 c S HS) as (Hc&H1). split; first done.
+  intros t L HL. specialize (H1 t L HL) as (Ht&H2). split; first done.
+  intros l ps Hl. eapply tag_protected_for_mono; last by eapply H2.
+  intros l' it ???. by eapply Hweak.
 Qed.
 
